@prefix : <https://w3id.org/def/dedl#> .
@prefix dc: <http://purl.org/dc/elements/1.1/> .
@prefix owl: <http://www.w3.org/2002/07/owl#> .
@prefix rdf: <http://www.w3.org/1999/02/22-rdf-syntax-ns#> .
@prefix xml: <http://www.w3.org/XML/1998/namespace> .
@prefix xsd: <http://www.w3.org/2001/XMLSchema#> .
@prefix dedl: <https://w3id.org/def/dedl#> .
@prefix didl: <https://w3id.org/def/didl#> .
@prefix rdfs: <http://www.w3.org/2000/01/rdf-schema#> .
@prefix dcterms: <http://purl.org/dc/terms/> .
@base <https://w3id.org/def/dedl#> .

<https://w3id.org/def/dedl> rdf:type owl:Ontology ;
                             dc:description "The Data Ecosystem Description Language (DEDL) is an abstract language to describe concepts of data ecosystems, in which different participants (i.e., organizations and individuals) share data and generate value as the primary aim."@en ;
                             dc:title "DEDL Vocabulary & Expression 0.2"@en ;
                             dcterms:creator "Lennart Kl√∂pper, Jiahang Chen" ;
                             rdfs:comment "This is a vocabulary for DEDL version 0.2"@en ;
                             rdfs:label "DEDL"@en ;
                             owl:versionInfo 0.2 .

#################################################################
#    Annotation properties
#################################################################

###  http://purl.org/dc/elements/1.1/description
dc:description rdf:type owl:AnnotationProperty .


###  http://purl.org/dc/elements/1.1/title
dc:title rdf:type owl:AnnotationProperty .


###  http://purl.org/dc/terms/abstract
dcterms:abstract rdf:type owl:AnnotationProperty .


###  http://purl.org/dc/terms/created
dcterms:created rdf:type owl:AnnotationProperty .


###  http://purl.org/dc/terms/creator
dcterms:creator rdf:type owl:AnnotationProperty .


###  http://purl.org/dc/terms/license
dcterms:license rdf:type owl:AnnotationProperty .


#################################################################
#    Object Properties
#################################################################

###  https://w3id.org/def/dedl#accessControlModel
dedl:accessControlModel rdf:type owl:ObjectProperty ;
                        rdfs:domain dedl:Policy ;
                        rdfs:range dedl:AccessControlModel ;
                        rdfs:comment "Associates a Policy with its AccessControlModel to define and enforce resource access rules."@en ;
                        rdfs:label "accessControlModel"@en .


###  https://w3id.org/def/dedl#authenticationFactor
dedl:authenticationFactor rdf:type owl:ObjectProperty ;
                          rdfs:domain dedl:Authenticator ;
                          rdfs:range dedl:AuthenticationFactor ;
                          rdfs:comment "Indicates the AuthenticationFactor that an Authenticator uses."@en ;
                          rdfs:label "authenticationFactor"@en .


###  https://w3id.org/def/dedl#authenticationProcess
dedl:authenticationProcess rdf:type owl:ObjectProperty ;
                           rdfs:domain dedl:Authenticator ;
                           rdfs:range dedl:Authentication ;
                           rdfs:comment "Links an Authenticator to the authentication process used for identity verification."@en ;
                           rdfs:label "authenticationProcess"@en .


###  https://w3id.org/def/dedl#authenticationProtocol
dedl:authenticationProtocol rdf:type owl:ObjectProperty ;
                            rdfs:domain dedl:Authenticator ;
                            rdfs:range dedl:AuthenticationProtocol ;
                            rdfs:comment "Specifies the AuthenticationProtocol an Authenticator follows."@en ;
                            rdfs:label "authenticationProtocol"@en .


###  https://w3id.org/def/dedl#authenticationRiskContext
dedl:authenticationRiskContext rdf:type owl:ObjectProperty ;
                               rdfs:domain dedl:Authenticator ;
                               rdfs:range dedl:AuthenticationRiskContext ;
                               rdfs:comment "Associates an Authenticator with contextual factors that influence authentication risk."@en ;
                               rdfs:label "authenticationRiskContext"@en .


###  https://w3id.org/def/dedl#authorizationArchitecture
dedl:authorizationArchitecture rdf:type owl:ObjectProperty ;
                               rdfs:domain dedl:Authorizator ;
                               rdfs:range dedl:AuthorizationArchitecture ;
                               rdfs:comment "Specifies the AuthorizationArchitecture used by an Authorizator."@en ;
                               rdfs:label "authorizationArchitecture"@en .


###  https://w3id.org/def/dedl#authorizationProcess
dedl:authorizationProcess rdf:type owl:ObjectProperty ;
                          rdfs:domain dedl:Authorizator ;
                          rdfs:range dedl:Authorization ;
                          rdfs:comment "Indicates the authorization process followed by an Authorizator."@en ;
                          rdfs:label "authorizationProcess"@en .

###  https://w3id.org/def/dedl#dataEcosystem
dedl:dataEcosystem rdf:type owl:ObjectProperty ;
            rdfs:domain dedl:DataEcosystem ;
            rdfs:range dedl:DataEcosystem ;
            rdfs:comment "Indicates if the data ecosystem consists of multiple data ecosystem"@en ;
            rdfs:label "dataEcosystem"@en ;
            rdfs:seeAlso "composedOf (Oliveira)"@en .			
###  https://w3id.org/def/dedl#dataEcosystemElement
dedl:dataEcosystemElement rdf:type owl:ObjectProperty ;
                          rdfs:domain dedl:DataEcosystem ;
                          rdfs:range dedl:DataEcosystemElement ;
                          rdfs:comment ""@en ;
                          rdfs:label "dataEcosystemElement"@en ;
                          rdfs:seeAlso "composedBy (Oliveira)"@en .


###  https://w3id.org/def/dedl#entity
dedl:entity rdf:type owl:ObjectProperty ;
            rdfs:domain dedl:Participant ;
            rdfs:range dedl:Entity ;
            rdfs:comment "Associates a Participant with a particular Entity in the data ecosystem."@en ;
            rdfs:label "entity"@en .


###  https://w3id.org/def/dedl#identity
dedl:identity rdf:type owl:ObjectProperty ;
              rdfs:domain dedl:Entity ;
              rdfs:range didl:Identity ;
              rdfs:comment "Indicates the Identity belonging to an Entity."@en ;
              rdfs:label "identity"@en .
###  https://w3id.org/def/dedl#memberOf
dedl:memberOf rdf:type owl:ObjectProperty ;
          rdfs:domain dedl:Participant ;
          rdfs:range dedl:Organization ;
          rdfs:label "memberOf"@en .
							 

###  https://w3id.org/def/dedl#operates
dedl:operates rdf:type owl:ObjectProperty ;
          rdfs:domain dedl:Participant ;
          rdfs:range dedl:TechnicalDataEcosystemElement ;
          rdfs:comment "Specifies an operator of a TechnicalDataEcosystemElement."@en ;
          rdfs:label "operates"@en .									   


###  https://w3id.org/def/dedl#operator
dedl:operator rdf:type owl:ObjectProperty ;
          rdfs:domain dedl:DataEcosystem ;
          rdfs:range dedl:Participant ;
          rdfs:comment "Specifies an operator of a DataEcosystem."@en ;
          rdfs:label "operator"@en .


###  https://w3id.org/def/dedl#participant
dedl:participant rdf:type owl:ObjectProperty ;
             rdfs:domain dedl:DataEcosystem ;
             rdfs:range dedl:Participant ;
             rdfs:isDefinedBy "Specifies a participant within a DataEcosystem."@en ;
             rdfs:label "participant"@en .

###  https://w3id.org/def/dedl#policy
dedl:policy rdf:type owl:ObjectProperty ;
            rdfs:domain dedl:Entity ;
            rdfs:range dedl:Policy ;
            rdfs:comment "Links an Entity to a Policy governing its usage or access rights."@en ;
            rdfs:label "policy"@en .


###  https://w3id.org/def/dedl#policyLanguage
dedl:policyLanguage rdf:type owl:ObjectProperty ;
                    rdfs:domain dedl:Policy ;
                    rdfs:range dedl:PolicyLanguage ;
                    rdfs:comment "Specifies the PolicyLanguage used to express or encode a Policy."@en ;
                    rdfs:label "policyLanguage"@en .


###  https://w3id.org/def/dedl#process
dedl:process rdf:type owl:ObjectProperty ;
             rdfs:domain dedl:DataEcosystem ;
             rdfs:range dedl:Process ;
             rdfs:comment "Associates a DataEcosystem with a particular Process."@en ;
             rdfs:label "process"@en .


###  https://w3id.org/def/dedl#uses
dedl:uses rdf:type owl:ObjectProperty ;
          rdfs:domain dedl:Participant ;
          rdfs:range dedl:TechnicalDataEcosystemElement ;
          rdfs:comment ""@en ;
          rdfs:label "uses"@en .


#################################################################
#    Classes
#################################################################

###  https://w3id.org/def/dedl#API
dedl:API rdf:type owl:Class ;
         rdfs:subClassOf dedl:Interface ;
         rdfs:comment "Application Programming Interface; a subclass of Interface representing a set of protocols allowing different software entities to communicate within a data ecosystem."@en ;
         rdfs:label "API"@en .


###  https://w3id.org/def/dedl#AccessControlModel
dedl:AccessControlModel rdf:type owl:Class ;
                        rdfs:comment "A conceptual framework defining how access to resources is managed, granted, and restricted."@en ;
                        rdfs:label "AccessControlModel"@en .


###  https://w3id.org/def/dedl#AgreementStorage
dedl:AgreementStorage rdf:type owl:Class ;
                      rdfs:subClassOf dedl:PolicyStorage ;
                      rdfs:comment "A subclass of PolicyStorage where concluded contracts are stored, ensuring that agreements between Participants are documented and accessible."@en ;
                      rdfs:label "AgreementStorage"@en .


###  https://w3id.org/def/dedl#AuditAndLogging
dedl:AuditAndLogging rdf:type owl:Class ;
                     rdfs:subClassOf dedl:TechnicalDataEcosystemElement ;
                     rdfs:comment "A component responsible for documenting activities within a data ecosystem to ensure transparency."@en ;
                     rdfs:label "AuditAndLogging"@en .


###  https://w3id.org/def/dedl#Authentication
dedl:Authentication rdf:type owl:Class ;
                    rdfs:subClassOf dedl:Process ;
                    rdfs:comment "A procedure or sequence of steps that verify the identity of a user or entity."@en ;
                    rdfs:label "Authentication"@en .


###  https://w3id.org/def/dedl#AuthenticationFactor
dedl:AuthenticationFactor rdf:type owl:Class ;
                          rdfs:comment "An element used to verify the identity of a user or entity (e.g. password, token, biometrics)."@en ;
                          rdfs:label "AuthenticationFactor"@en .


###  https://w3id.org/def/dedl#AuthenticationProtocol
dedl:AuthenticationProtocol rdf:type owl:Class ;
                            rdfs:comment "A specification of the interactions or steps used to perform authentication."@en ;
                            rdfs:label "AuthenticationProtocol"@en .


###  https://w3id.org/def/dedl#AuthenticationRiskContext
dedl:AuthenticationRiskContext rdf:type owl:Class ;
                               rdfs:comment "Contextual attributes (time, location, device) that affect authentication risk levels."@en ;
                               rdfs:label "AuthenticationRiskContext"@en .


###  https://w3id.org/def/dedl#Authenticator
dedl:Authenticator rdf:type owl:Class ;
                   rdfs:subClassOf dedl:IdentityAndAccessManagement ;
                   rdfs:comment "An Participant or component responsible for carrying out the authentication process."@en ;
                   rdfs:label "Authenticator"@en .


###  https://w3id.org/def/dedl#Authorization
dedl:Authorization rdf:type owl:Class ;
                   rdfs:subClassOf dedl:Process ;
                   rdfs:comment "A method or set of steps determining if an entity may access a resource."@en ;
                   rdfs:label "Authorization"@en .


###  https://w3id.org/def/dedl#AuthorizationArchitecture
dedl:AuthorizationArchitecture rdf:type owl:Class ;
                               rdfs:comment "A subclass of IdentityAndAccessManagement representing a structural framework that defines how authorization decisions are made and enforced."@en ;
                               rdfs:label "AuthorizationArchitecture"@en .


###  https://w3id.org/def/dedl#Authorizator
dedl:Authorizator rdf:type owl:Class ;
                  rdfs:subClassOf dedl:IdentityAndAccessManagement ;
                  rdfs:comment "A participant or component that assesses permissions and enforces authorization decisions."@en ;
                  rdfs:label "Authorizator"@en .


###  https://w3id.org/def/dedl#Communication
dedl:Communication rdf:type owl:Class ;
                   rdfs:subClassOf dedl:TechnicalDataEcosystemElement ;
                   rdfs:comment "A mechanism through which participants in a data ecosystem exchange information and interact with each other."@en ;
                   rdfs:label "Communication"@en .


###  https://w3id.org/def/dedl#ContractAgreeing
dedl:ContractAgreeing rdf:type owl:Class ;
                      rdfs:subClassOf dedl:Negotiating ;
                      rdfs:comment "A subclass of Negotiation representing the concluding process between data providers and consumers  when a policy is accepted by both parties and a contract is formed."@en ;
                      rdfs:label "ContractAgreeing"@en .


###  https://w3id.org/def/dedl#ContractOffering
dedl:ContractOffering rdf:type owl:Class ;
                      rdfs:subClassOf dedl:Negotiating ;
                      rdfs:comment "A subclass of Negotiating representing the process where data offers are made available to potential consumers."@en ;
                      rdfs:label "ContractOffering"@en .


###  https://w3id.org/def/dedl#ContractRequesting
dedl:ContractRequesting rdf:type owl:Class ;
                        rdfs:subClassOf dedl:Negotiating ;
                        rdfs:comment "A subclass of Negotiating representing the process where potential data consumers request specific conditions for the use or access of data."@en ;
                        rdfs:label "ContractRequesting"@en .


###  https://w3id.org/def/dedl#DataEcosystem
dedl:DataEcosystem rdf:type owl:Class ;
                   rdfs:comment "A socio-technical system in which participants share and manage data and associated processes."@en ;
                   rdfs:label "DataEcosystem"@en .


###  https://w3id.org/def/dedl#DataEcosystemElement
dedl:DataEcosystemElement rdf:type owl:Class ;
                          rdfs:comment "An element within a data ecosystem that contributes to its functionality and processes."@en ;
                          rdfs:label "DataEcosystemElement"@en .


###  https://w3id.org/def/dedl#DataExchanging
dedl:DataExchanging rdf:type owl:Class ;
                    rdfs:subClassOf dedl:Transacting ;
                    rdfs:comment "A subclass of Transaction that represents the process that facilitates the transfer of data within a data ecosystem between Participants."@en ;
                    rdfs:label "DataExchanging"@en .


###  https://w3id.org/def/dedl#DataOffering
dedl:DataOffering rdf:type owl:Class ;
                  rdfs:subClassOf dedl:Publishing ;
                  rdfs:comment "A sublcass of Publishing representing the process where participants make their data available to others in the data ecosystem."@en ;
                  rdfs:label "DataOffering"@en .


###  https://w3id.org/def/dedl#DataSpaceConnector
dedl:DataSpaceConnector rdf:type owl:Class ;
                        rdfs:subClassOf dedl:Interface ;
                        rdfs:comment "A subclass of Interface enabling secure and standardized interaction within data spaces (i.e., specialized realizations of data ecosystems)."@en ;
                        rdfs:label "DataSpaceConnector"@en .


###  https://w3id.org/def/dedl#DataStorage
dedl:DataStorage rdf:type owl:Class ;
                 rdfs:subClassOf dedl:Storage ;
                 rdfs:comment "A subclass of Storage dedicated to string data within a data ecosystem."@en ;
                 rdfs:label "DataStorage"@en .


###  https://w3id.org/def/dedl#DataStoring
dedl:DataStoring rdf:type owl:Class ;
                 rdfs:subClassOf dedl:Publishing ;
                 rdfs:comment "A subclass of Publishing representing the process that ensures datasets are stored securely, either centrally or decentrally, depending on the architecture of the data ecosystem."@en ;
                 rdfs:label "DataStoring"@en .


###  https://w3id.org/def/dedl#Decision
dedl:Decision rdf:type owl:Class ;
              rdfs:comment "An outcome regarding an authorization request, e.g. Allow or Deny."@en ;
              rdfs:label "Decision"@en .


###  https://w3id.org/def/dedl#Entity
dedl:Entity rdf:type owl:Class ;
            rdfs:comment "Any identifiable object of a participant within the data ecosystem, e.g. a device or digital resource."@en ;
            rdfs:label "Entity"@en .


###  https://w3id.org/def/dedl#Finding
dedl:Finding rdf:type owl:Class ;
             rdfs:subClassOf dedl:Process ;
             rdfs:comment "An optional process that enables information or data to be found within a data ecosystem."@en ;
             rdfs:label "Finding"@en .


###  https://w3id.org/def/dedl#GUI
dedl:GUI rdf:type owl:Class ;
         rdfs:subClassOf dedl:Interface ;
         rdfs:comment "Graphical User Interface; a subclass of Interface representing an interface through which users can visually interact with components of a data ecosystem."@en ;
         rdfs:label "GUI"@en .


###  https://w3id.org/def/dedl#IdentityAndAccessManagement
dedl:IdentityAndAccessManagement rdf:type owl:Class ;
                                 rdfs:subClassOf dedl:TechnicalDataEcosystemElement ;
                                 rdfs:comment "A framework ensuring that only authorized Participants have access to a data ecosystem."@en ;
                                 rdfs:label "IdentityAndAccessManagement"@en .


###  https://w3id.org/def/dedl#IdentityProvider
dedl:IdentityProvider rdf:type owl:Class ;
                      rdfs:subClassOf dedl:IdentityAndAccessManagement ;
                      rdfs:comment "A subclass of IdentityAndAccessManagement representing a component responsible for managing digital identities, facilitating onboarding and offboarding processes in a data ecosystem."@en ;
                      rdfs:label "IdentityProvider"@en .


###  https://w3id.org/def/dedl#Individual
dedl:Individual rdf:type owl:Class ;
                rdfs:subClassOf dedl:Participant ;
                rdfs:comment "A subclass of Participant representing a legal person."@en ;
                rdfs:label "Individual"@en .


###  https://w3id.org/def/dedl#Interface
dedl:Interface rdf:type owl:Class ;
               rdfs:subClassOf dedl:TechnicalDataEcosystemElement ;
               rdfs:comment "An access point for participants to join and interact within a data ecosystem."@en ;
               rdfs:label "Interface"@en .


###  https://w3id.org/def/dedl#Negotiating
dedl:Negotiating rdf:type owl:Class ;
                 rdfs:subClassOf dedl:Process ;
                 rdfs:comment "An optional process where participants discuss and agree on policies leading to contracts within a data ecosystem."@en ;
                 rdfs:label "Negotiating"@en .


###  https://w3id.org/def/dedl#Offboarding
dedl:Offboarding rdf:type owl:Class ;
                 rdfs:subClassOf dedl:Process .


###  https://w3id.org/def/dedl#OfferStorage
dedl:OfferStorage rdf:type owl:Class ;
                  rdfs:subClassOf dedl:PolicyStorage ;
                  rdfs:comment "A subclass of PolicyStorage where data offers are stored, allowing participants in a data ecosystem to publish and manage their available datasets or services."@en ;
                  rdfs:label "OfferStorage"@en .


###  https://w3id.org/def/dedl#Onboarding
dedl:Onboarding rdf:type owl:Class ;
                rdfs:subClassOf dedl:Process .


###  https://w3id.org/def/dedl#Organization
dedl:Organization rdf:type owl:Class ;
                  rdfs:subClassOf dedl:Participant ;
                  rdfs:comment "A subclass of Participant representing a legal entity."@en ;
                  rdfs:label "Organization"@en .


###  https://w3id.org/def/dedl#Participant
dedl:Participant rdf:type owl:Class ;
                 rdfs:subClassOf dedl:DataEcosystemElement ;
                 rdfs:comment "A stakeholder participating in or operating the data ecosystem (either an Individual or Organization)."@en ;
                 rdfs:label "Participant"@en .


###  https://w3id.org/def/dedl#Policy
dedl:Policy rdf:type owl:Class ;
            rdfs:comment "A set of rules or guidelines that govern data usage, sharing, and access."@en ;
            rdfs:label "Policy"@en .


###  https://w3id.org/def/dedl#PolicyLanguage
dedl:PolicyLanguage rdf:type owl:Class ;
                    rdfs:comment "A formal language for defining and expressing policies."@en ;
                    rdfs:label "PolicyLanguage"@en .


###  https://w3id.org/def/dedl#PolicyStorage
dedl:PolicyStorage rdf:type owl:Class ;
                   rdfs:subClassOf dedl:Storage ;
                   rdfs:comment "A subclass of storage that stores the conditions under which access to resources in a data ecosystem is granted and how they may be used."@en ;
                   rdfs:label "PolicyStorage"@en .


###  https://w3id.org/def/dedl#Process
dedl:Process rdf:type owl:Class ;
             rdfs:comment "A series of operations or activities performed within the data ecosystem."@en ;
             rdfs:label "Process"@en .


###  https://w3id.org/def/dedl#Publishing
dedl:Publishing rdf:type owl:Class ;
                rdfs:subClassOf dedl:Process ;
                rdfs:comment "An optional process that makes data discoverable and allows its findability through catalogs or metadata integration."@en ;
                rdfs:label "Publishing"@en .


###  https://w3id.org/def/dedl#RunTimeEnvironment
dedl:RunTimeEnvironment rdf:type owl:Class ;
                        rdfs:subClassOf dedl:TechnicalDataEcosystemElement ;
                        rdfs:comment "An infrastructure required for executing services within a data ecosystem, providing the necessary computing resources."@en ;
                        rdfs:label "RunTimeEnvironment"@en .


###  https://w3id.org/def/dedl#Service
dedl:Service rdf:type owl:Class ;
             rdfs:subClassOf dedl:TechnicalDataEcosystemElement ;
             rdfs:comment "A service developed to address specific needs within a data ecosystem, often involving data processing or visualization."@en ;
             rdfs:label "Service" .


###  https://w3id.org/def/dedl#ServiceExecuting
dedl:ServiceExecuting rdf:type owl:Class ;
                      rdfs:subClassOf dedl:Transacting ;
                      rdfs:comment "A  subclass of Transaction representing the process that enables third-party services execution to generate additional value from the managed data in a data ecosystem."@en ;
                      rdfs:label "ServiceExecuting"@en .


###  https://w3id.org/def/dedl#Storage
dedl:Storage rdf:type owl:Class ;
             rdfs:subClassOf dedl:TechnicalDataEcosystemElement ;
             rdfs:comment "A component where various types of information are stored in a data ecosystem."@en ;
             rdfs:label "Storage"@en .


###  https://w3id.org/def/dedl#TechnicalDataEcosystemElement
dedl:TechnicalDataEcosystemElement rdf:type owl:Class ;
                                   rdfs:subClassOf dedl:DataEcosystemElement ;
                                   rdfs:comment "A subclass of DataEcosystemElement focused on technical components necessary for the operation of a data ecosystem."@en ;
                                   rdfs:label "TechnicalDataEcosystemElement"@en .


###  https://w3id.org/def/dedl#Transacting
dedl:Transacting rdf:type owl:Class ;
                 rdfs:subClassOf dedl:Process ;
                 rdfs:comment "A mandatory process that enables the exchange or transfer of data or other resources between Participants within a data ecosystem."@en ;
                 rdfs:label "Transacting"@en .


###  https://w3id.org/def/didl#Identity
didl:Identity rdf:type owl:Class ;
              rdfs:comment "A unique collection of attributes, credentials, or characteristics of an entity."@en ;
              rdfs:label "Identity"@en .


#################################################################
#    Individuals
#################################################################

###  https://w3id.org/def/dedl#ABAC
dedl:ABAC rdf:type owl:NamedIndividual ,
                   dedl:AccessControlModel ;
          rdfs:comment "Attribute-based Access Control model, relying on attributes to define permissions."@en ;
          rdfs:label "ABAC"@en .


###  https://w3id.org/def/dedl#ACP
dedl:ACP rdf:type owl:NamedIndividual ,
                  dedl:PolicyLanguage ;
         rdfs:comment "Access control policy language (ACP), a particular set of grammar, syntax rules (logical and mathematical), and operators which provides an abstraction-layer for access control policy specifications, see https://solid.github.io/authorization-panel/acp-specification/"@en ;
         rdfs:label "ACP"@en .


###  https://w3id.org/def/dedl#Allow
dedl:Allow rdf:type owl:NamedIndividual ,
                    dedl:Decision ;
           rdfs:comment "A Decision indicating that access is permitted."@en ;
           rdfs:label "Allow"@en .


###  https://w3id.org/def/dedl#Behavior
dedl:Behavior rdf:type owl:NamedIndividual ,
                       dedl:AuthenticationRiskContext ;
              rdfs:comment "A context factor reflecting user behavioral patterns (e.g., keystroke dynamics)."@en ;
              rdfs:label "Behavior"@en .


###  https://w3id.org/def/dedl#CapBAC
dedl:CapBAC rdf:type owl:NamedIndividual ,
                     dedl:AccessControlModel ;
            rdfs:comment "Capability-based Access Control relying on tokens or 'capabilities' to grant permissions."@en ;
            rdfs:label "CapBAC"@en .


###  https://w3id.org/def/dedl#Cryptography
dedl:Cryptography rdf:type owl:NamedIndividual ,
                           dedl:AuthenticationProtocol ;
                  rdfs:comment "An authentication protocol leveraging cryptographic techniques to prove identity."@en ;
                  rdfs:label "Cryptography"@en .


###  https://w3id.org/def/dedl#DAC
dedl:DAC rdf:type owl:NamedIndividual ,
                  dedl:AccessControlModel ;
         rdfs:comment "Discretionary Access Control, where resource owners grant or deny permissions."@en ;
         rdfs:label "DAC"@en .


###  https://w3id.org/def/dedl#Deny
dedl:Deny rdf:type owl:NamedIndividual ,
                   dedl:Decision ;
          rdfs:comment "A Decision indicating that access is refused."@en ;
          rdfs:label "Deny"@en .


###  https://w3id.org/def/dedl#Device
dedl:Device rdf:type owl:NamedIndividual ,
                     dedl:AuthenticationRiskContext ;
            rdfs:comment "A factor in the authentication risk context indicating the device used for login."@en ;
            rdfs:label "Device"@en .


###  https://w3id.org/def/dedl#Geolocation
dedl:Geolocation rdf:type owl:NamedIndividual ,
                          dedl:AuthenticationRiskContext ;
                 rdfs:comment "A factor in the authentication risk context representing physical or network location."@en ;
                 rdfs:label "Geolocation"@en .


###  https://w3id.org/def/dedl#HybridArchitecture
dedl:HybridArchitecture rdf:type owl:NamedIndividual ,
                                 dedl:AuthorizationArchitecture ;
                        rdfs:comment "An AuthorizationArchitecture combining policy-based and token-based architecture"@en ;
                        rdfs:label "HybridArchitecture"@en .


###  https://w3id.org/def/dedl#Kerberos
dedl:Kerberos rdf:type owl:NamedIndividual ,
                       dedl:AuthenticationProtocol ;
              rdfs:comment "A protocol using a trusted third-party ticket-granting service for authentication."@en ;
              rdfs:label "Kerberos"@en .


###  https://w3id.org/def/dedl#LDAP
dedl:LDAP rdf:type owl:NamedIndividual ,
                   dedl:AuthenticationProtocol ;
          rdfs:comment "Lightweight Directory Access Protocol, often used to manage authentication data in directories."@en ;
          rdfs:label "LDAP"@en .


###  https://w3id.org/def/dedl#MAC
dedl:MAC rdf:type owl:NamedIndividual ,
                  dedl:AccessControlModel ;
         rdfs:comment "Mandatory Access Control, where policies are enforced by a central authority."@en ;
         rdfs:label "MAC"@en .


###  https://w3id.org/def/dedl#MPEG-21
dedl:MPEG-21 rdf:type owl:NamedIndividual ,
                      dedl:PolicyLanguage ;
             rdfs:comment "A digital rights management and usage rights framework which can serve as a policy language."@en ;
             rdfs:label "MPEG-21"@en .


###  https://w3id.org/def/dedl#MultiFactor
dedl:MultiFactor rdf:type owl:NamedIndividual ,
                          dedl:AuthenticationFactor ;
                 rdfs:comment "An authentication factor requiring two or more independent credentials."@en ;
                 rdfs:label "MultiFactor"@en .


###  https://w3id.org/def/dedl#Negotiate
dedl:Negotiate rdf:type owl:NamedIndividual ,
                        dedl:Authorization ;
               rdfs:comment "An authorization process involving negotiation or exchange of data before deciding access."@en ;
               rdfs:label "Negotiate"@en .


###  https://w3id.org/def/dedl#OBAC
dedl:OBAC rdf:type owl:NamedIndividual ,
                   dedl:AccessControlModel ;
          rdfs:comment "Ontology-based Access Control focusing on contextual policy enforcement"@en ;
          rdfs:label "OBAC"@en .


###  https://w3id.org/def/dedl#ODRL
dedl:ODRL rdf:type owl:NamedIndividual ,
                   dedl:PolicyLanguage ;
          rdfs:comment "Open Digital Rights Language, commonly used to specify rights, constraints, and obligations."@en ;
          rdfs:label "ODRL"@en .


###  https://w3id.org/def/dedl#OIDC
dedl:OIDC rdf:type owl:NamedIndividual ,
                   dedl:AuthenticationProtocol ;
          rdfs:comment "OpenID Connect, a simple identity layer built on OAuth 2.0 used for single sign-on."@en ;
          rdfs:label "OIDC"@en .


###  https://w3id.org/def/dedl#OneWay
dedl:OneWay rdf:type owl:NamedIndividual ,
                     dedl:Authentication ;
            rdfs:comment "A one-direction authentication process, typically from a client to a server."@en ;
            rdfs:label "OneWay"@en .


###  https://w3id.org/def/dedl#OrBAC
dedl:OrBAC rdf:type owl:NamedIndividual ,
                    dedl:AccessControlModel ;
           rdfs:comment "Organization-based Access Control, focusing on roles and contexts within an organization."@en ;
           rdfs:label "OrBAC"@en .


###  https://w3id.org/def/dedl#PolicyBasedArchitecture
dedl:PolicyBasedArchitecture rdf:type owl:NamedIndividual ,
                                      dedl:AuthorizationArchitecture ;
                             rdfs:comment "An AuthorizationArchitecture where authorization relies on evaluating formalized policies."@en ;
                             rdfs:label "PolicyBasedArchitecture"@en .


###  https://w3id.org/def/dedl#Poll
dedl:Poll rdf:type owl:NamedIndividual ,
                   dedl:Authorization ;
          rdfs:comment "An authorization process where a client periodically checks the server for an access decision."@en ;
          rdfs:label "Poll"@en .


###  https://w3id.org/def/dedl#Ponder
dedl:Ponder rdf:type owl:NamedIndividual ,
                     dedl:PolicyLanguage ;
            rdfs:comment "A policy specification language for security and management in distributed systems."@en ;
            rdfs:label "Ponder"@en .


###  https://w3id.org/def/dedl#Push
dedl:Push rdf:type owl:NamedIndividual ,
                   dedl:Authorization ;
          rdfs:comment "An authorization process where the server proactively notifies the client about decisions."@en ;
          rdfs:label "Push"@en .


###  https://w3id.org/def/dedl#RBAC
dedl:RBAC rdf:type owl:NamedIndividual ,
                   dedl:AccessControlModel ;
          rdfs:comment "Role-based Access Control, assigning permissions to roles which are then assigned to users."@en ;
          rdfs:label "RBAC"@en .


###  https://w3id.org/def/dedl#Rego
dedl:Rego rdf:type owl:NamedIndividual ,
                   dedl:PolicyLanguage ;
          rdfs:comment "A declarative policy language used with Open Policy Agent (OPA) to define fine-grained permissions."@en ;
          rdfs:label "Rego"@en .


###  https://w3id.org/def/dedl#RightsML
dedl:RightsML rdf:type owl:NamedIndividual ,
                       dedl:PolicyLanguage ;
              rdfs:comment "An ODRL-based language for expressing rights and usage constraints, common in news/media."@en ;
              rdfs:label "RightsML"@en .


###  https://w3id.org/def/dedl#SAML_2.0
dedl:SAML_2.0 rdf:type owl:NamedIndividual ,
                       dedl:AuthenticationProtocol ;
              rdfs:comment "Security Assertion Markup Language (2.0), exchanging authentication and authorization data."@en ;
              rdfs:label "SAML2.0"@en .


###  https://w3id.org/def/dedl#Signature
dedl:Signature rdf:type owl:NamedIndividual ,
                        dedl:AuthenticationProtocol ;
               rdfs:comment "An authentication protocol relying on digital signatures for verification."@en ;
               rdfs:label "Signature"@en .


###  https://w3id.org/def/dedl#SingleFactor
dedl:SingleFactor rdf:type owl:NamedIndividual ,
                           dedl:AuthenticationFactor ;
                  rdfs:comment "An authentication factor using only one method of verification (e.g., a single password)."@en ;
                  rdfs:label "SingleFactor"@en .


###  https://w3id.org/def/dedl#ThreeWay
dedl:ThreeWay rdf:type owl:NamedIndividual ,
                       dedl:Authentication ;
              rdfs:comment "An authentication process involving a three-part handshake or three-step verification."@en ;
              rdfs:label "ThreeWay"@en .


###  https://w3id.org/def/dedl#Time-based
dedl:Time-based rdf:type owl:NamedIndividual ,
                         dedl:AuthenticationRiskContext ;
                rdfs:comment "A context factor referencing time-sensitive credentials or restrictions (e.g., OTPs)."@en ;
                rdfs:label "TimeBased"@en .


###  https://w3id.org/def/dedl#TokenBasedArchitecture
dedl:TokenBasedArchitecture rdf:type owl:NamedIndividual ,
                                     dedl:AuthorizationArchitecture ;
                            rdfs:comment "An authorization architecture using tokens (e.g., JWT)"@en ;
                            rdfs:label "TokenBasedArchitecture"@en .


###  https://w3id.org/def/dedl#TwoWay
dedl:TwoWay rdf:type owl:NamedIndividual ,
                     dedl:Authentication ;
            rdfs:comment "A mutual authentication process where both parties verify each other's identity."@en ;
            rdfs:label "TwoWay"@en .


###  https://w3id.org/def/dedl#WebAuth
dedl:WebAuth rdf:type owl:NamedIndividual ,
                      dedl:AuthenticationProtocol ;
             rdfs:comment "A web-based authentication protocol, encompassing flows like OAuth, SAML, or WebAuthn."@en ;
             rdfs:label "WebAuth"@en .


###  https://w3id.org/def/dedl#XACMLPolicyLanguage
dedl:XACMLPolicyLanguage rdf:type owl:NamedIndividual ,
                                  dedl:PolicyLanguage ;
                         rdfs:comment "An OASIS standard policy language for defining access control rules (XACML framework)."@en ;
                         rdfs:label "XACMLPolicyLanguage"@en .


###  Generated by the OWL API (version 4.5.29.2024-05-13T12:11:03Z) https://github.com/owlcs/owlapi
